theories/Runtime/SmallStepPaperTheorems.v
@@ -1,4 +1,5 @@
 From stdpp Require Import gmap.
+From Stdlib Require Import Program.Equality.
 
 Require Import theories.Runtime.Heap.
 Require Import theories.Runtime.HeapTyping.
@@ -12,6 +13,7 @@ Require Import theories.Runtime.SmallStepRuntimeKontTyping.
 Require Import theories.Runtime.SmallStepRuntimeStateShape.
 Require Import theories.Runtime.SmallStepPreservationTheorems.
 Require Import theories.Runtime.SmallStepExplicitStoreBase.
+Require Import theories.Runtime.SmallStepExplicitStoreTheorems.
 Require Import theories.Runtime.SmallStepTraceSafety.
 Require Import theories.Runtime.SmallStepParallelTraceSafe.
 Require Import theories.Runtime.SmallStepSequentialSoundness.
@@ -209,6 +211,248 @@ Proof.
   exact PairParCheckedStructuredStepsPhi_top_sound.
 Qed.
 
+Theorem PaperPairParCheckedPackedTerminalSoundness :
+  forall heap env rho ef1 ea1 ef2 ea2 k stty ctxt rgns
+    ty1 ty2 eff1 eff2 tout phi heap' v theta1 theta2,
+    TcHeap (heap, stty) ->
+    RuntimeHeapShape heap stty ->
+    TcRho (rho, rgns) ->
+    TcInc (ctxt, rgns) ->
+    TcEnv (stty, rho, env, ctxt) ->
+    RuntimeEnvShape stty rho env ctxt ->
+    TcExp (ctxt, rgns, Mu_App ef1 ea1, ty1, eff1) ->
+    TcExp (ctxt, rgns, Mu_App ef2 ea2, ty2, eff2) ->
+    WTKontRuntime stty (subst_rho rho (Ty_Pair ty1 ty2)) tout k ->
+    PairParCheckedPackedStepsPhi theta1 theta2
+      (pairpar_checked_start heap env rho ef1 ea1 ef2 ea2 k)
+      phi
+      (PPS_State (StDone heap' v)) ->
+    exists stty',
+      StoreExtends stty stty' /\
+      TcHeap (heap', stty') /\
+      RuntimeHeapShape heap' stty' /\
+      TcVal (stty', v, tout) /\
+      RuntimeValShape stty' tout v /\
+      TcPhi stty' phi.
+Proof.
+  exact PairParCheckedPackedStepsPhi_terminal_value_with_trace.
+Qed.
+
+Theorem PaperScheduledSmallStepTerminalValueSoundness :
+  forall state tout stty phi heap' v,
+    WTStateRuntimeHeapShapeAt state tout stty ->
+    ScheduledStepsPhi state phi (StDone heap' v) ->
+    exists stty',
+      StoreExtends stty stty' /\
+      TcHeap (heap', stty') /\
+      RuntimeHeapShape heap' stty' /\
+      TcVal (stty', v, tout) /\
+      RuntimeValShape stty' tout v.
+Proof.
+  exact WTStateRuntimeHeapShapeAt_scheduled_terminal_value.
+Qed.
+
+Lemma TcExp_mu_app_summary_readonly :
+  forall ctxt rgns rho ef ea ty static,
+    TcExp (ctxt, rgns, Mu_App ef ea, ty, static) ->
+    exists static_eff,
+      TcExp (ctxt, rgns, Eff_App ef ea, Ty_Effect, static_eff) /\
+      ReadOnlyStatic (fold_subst_eps rho static_eff).
+Proof.
+  intros ctxt rgns rho ef ea ty static HTcMu.
+  inversion HTcMu; subst.
+  match goal with
+  | HBackAll : forall rho0,
+      BackTriangle (ctxt, rgns, rho0, Mu_App ef ea, Eff_App ef ea) |- _ =>
+      pose proof (HBackAll rho) as HBack
+  end.
+  inversion HBack; subst; try solve [discriminate].
+  exists static_ee.
+  split.
+  - inversion H11; subst. exact H11.
+  - exact H12.
+Qed.
+
+Lemma PairParEffectSummaryStepsPhi_readonly_from_pairpar_typed :
+  forall heap env rho ef1 ea1 ef2 ea2 stty ctxt rgns ty static
+    phi_eff1 phi_eff2 heap_eff1 theta1 heap_eff2 theta2,
+    TcHeap (heap, stty) ->
+    RuntimeHeapShape heap stty ->
+    TcRho (rho, rgns) ->
+    TcInc (ctxt, rgns) ->
+    TcEnv (stty, rho, env, ctxt) ->
+    RuntimeEnvShape stty rho env ctxt ->
+    TcExp (ctxt, rgns, Pair_Par ef1 ea1 ef2 ea2, ty, static) ->
+    PairParEffectSummaryStepsPhi
+      heap env rho ef1 ea1 ef2 ea2
+      phi_eff1 phi_eff2 heap_eff1 theta1 heap_eff2 theta2 ->
+    ReadOnlyPhi phi_eff1 /\ ReadOnlyPhi phi_eff2.
+Proof.
+  intros heap env rho ef1 ea1 ef2 ea2 stty ctxt rgns ty static
+    phi_eff1 phi_eff2 heap_eff1 theta1 heap_eff2 theta2
+    HTcHeap HHeapShape HTcRho HTcInc HTcEnv HEnvShape HTcPair HSummary.
+  inversion HTcPair; subst.
+  match goal with
+  | HMu1 : TcExp (ctxt, rgns, Mu_App ef1 ea1, _, _),
+    HMu2 : TcExp (ctxt, rgns, Mu_App ef2 ea2, _, _) |- _ =>
+      destruct (TcExp_mu_app_summary_readonly
+        ctxt rgns rho ef1 ea1 _ _ HMu1)
+        as (static_eff1 & HTcEff1 & HReadOnly1);
+      destruct (TcExp_mu_app_summary_readonly
+        ctxt rgns rho ef2 ea2 _ _ HMu2)
+        as (static_eff2 & HTcEff2 & HReadOnly2);
+      exact
+        (PairParEffectSummaryStepsPhi_readonly_from_small_step_sound
+          heap env rho ef1 ea1 ef2 ea2 stty ctxt rgns
+          phi_eff1 phi_eff2 heap_eff1 theta1 heap_eff2 theta2
+          static_eff1 static_eff2
+          HTcHeap HHeapShape HTcRho HTcInc HTcEnv HEnvShape
+          HTcEff1 HTcEff2 HSummary HReadOnly1 HReadOnly2)
+  end.
+Qed.
+
+Theorem WTStateRuntimeHeapShapeAt_scheduled_terminal_value_with_trace :
+  forall state tout stty phi heap' v,
+    WTStateRuntimeHeapShapeAt state tout stty ->
+    ScheduledStepsPhi state phi (StDone heap' v) ->
+    exists stty',
+      StoreExtends stty stty' /\
+      TcHeap (heap', stty') /\
+      RuntimeHeapShape heap' stty' /\
+      TcVal (stty', v, tout) /\
+      RuntimeValShape stty' tout v /\
+      TcPhi stty' phi.
+Proof.
+  intros state tout stty phi heap' v HWT HSteps.
+  revert tout stty HWT.
+  dependent induction HSteps; intros tout stty HWT.
+  - destruct (WTStateRuntimeHeapShapeAt_done_value heap' v tout stty HWT)
+      as (HTcHeap & HHeapShape & HTcVal & HValShape).
+    exists stty.
+    split; [apply StoreExtends_refl |].
+    split; [exact HTcHeap |].
+    split; [exact HHeapShape |].
+    split; [exact HTcVal |].
+    split; [exact HValShape | apply TcPhi_nil].
+  - destruct
+      (WTStateRuntimeHeapShapeAt_step_preservation
+        state tout stty label state' HWT H0)
+      as (stty1 & HWT1 & _ & _ & HExt1).
+    destruct (IHHSteps heap' v eq_refl tout stty1 HWT1)
+      as (stty2 & HExt2 & HTcHeap2 & HHeapShape2 &
+          HTcVal2 & HValShape2 & HTcPhi2).
+    pose proof
+      (WTStateRuntimeHeapShapeAt_step_label_phi_typed
+        state tout stty label state' tout stty1 HWT H0 HWT1)
+      as HTcLabel1.
+    pose proof
+      (TcPhi_weaken stty1 stty2 (label_phi label) HExt2 HTcLabel1)
+      as HTcLabel2.
+    exists stty2.
+    split; [eapply StoreExtends_trans; eauto |].
+    split; [exact HTcHeap2 |].
+    split; [exact HHeapShape2 |].
+    split; [exact HTcVal2 |].
+    split; [exact HValShape2 |].
+    apply TcPhi_seq; assumption.
+  - inversion HWT; subst.
+    match goal with
+    | HTcExp : TcExp (_, _, Pair_Par _ _ _ _, _, _) |- _ =>
+        inversion HTcExp; subst
+    end.
+    destruct
+      (PairParCheckedPackedStepsPhi_terminal_value_with_trace
+        heap env rho ef1 ea1 ef2 ea2 k stty ctxt rgns
+        ty1 ty2 eff1 eff2 tout phi_mu heap' v theta1 theta2)
+      as (stty' & HExt & HTcHeap' & HHeapShape' & HTcVal' &
+          HValShape' & HTcPhiMu);
+      eauto.
+    destruct
+      (PairParEffectSummaryStepsPhi_readonly_from_pairpar_typed
+        heap env rho ef1 ea1 ef2 ea2 stty ctxt rgns
+        (Ty_Pair ty1 ty2)
+        (Union_Static_Action
+          (Union_Static_Action (Union_Static_Action eff3 eff4) eff2) eff1)
+        phi_eff1 phi_eff2 heap_eff1 theta1 heap_eff2 theta2)
+      as (HReadOnlyEff1 & HReadOnlyEff2);
+      eauto.
+    exists stty'.
+    split; [exact HExt |].
+    split; [exact HTcHeap' |].
+    split; [exact HHeapShape' |].
+    split; [exact HTcVal' |].
+    split; [exact HValShape' |].
+    apply TcPhi_pairpar_checked_packed_structured_trace.
+    + apply ReadOnlyPhi_TcPhi. exact HReadOnlyEff1.
+    + apply ReadOnlyPhi_TcPhi. exact HReadOnlyEff2.
+    + exact HTcPhiMu.
+Qed.
+
+Theorem PaperScheduledSmallStepTerminalTraceSoundness :
+  forall state tout stty phi heap' v,
+    WTStateRuntimeHeapShapeAt state tout stty ->
+    ScheduledStepsPhi state phi (StDone heap' v) ->
+    exists stty',
+      StoreExtends stty stty' /\
+      TcHeap (heap', stty') /\
+      RuntimeHeapShape heap' stty' /\
+      TcVal (stty', v, tout) /\
+      RuntimeValShape stty' tout v /\
+      TcPhi stty' phi.
+Proof.
+  exact WTStateRuntimeHeapShapeAt_scheduled_terminal_value_with_trace.
+Qed.
+
+Theorem PaperScheduledExpressionTerminalValueSoundness :
+  forall heap env rho e stty ctxt rgns t eff phi heap' v,
+    TcHeap (heap, stty) ->
+    RuntimeHeapShape heap stty ->
+    TcRho (rho, rgns) ->
+    TcInc (ctxt, rgns) ->
+    TcEnv (stty, rho, env, ctxt) ->
+    RuntimeEnvShape stty rho env ctxt ->
+    TcExp (ctxt, rgns, e, t, eff) ->
+    ScheduledStepsPhi
+      (initial_state heap env rho e)
+      phi
+      (StDone heap' v) ->
+    exists stty',
+      StoreExtends stty stty' /\
+      TcHeap (heap', stty') /\
+      RuntimeHeapShape heap' stty' /\
+      TcVal (stty', v, subst_rho rho t) /\
+      RuntimeValShape stty' (subst_rho rho t) v.
+Proof.
+  exact initial_state_scheduled_terminal_value.
+Qed.
+
+Theorem PaperScheduledExpressionTerminalTraceSoundness :
+  forall heap env rho e stty ctxt rgns t eff phi heap' v,
+    TcHeap (heap, stty) ->
+    RuntimeHeapShape heap stty ->
+    TcRho (rho, rgns) ->
+    TcInc (ctxt, rgns) ->
+    TcEnv (stty, rho, env, ctxt) ->
+    RuntimeEnvShape stty rho env ctxt ->
+    TcExp (ctxt, rgns, e, t, eff) ->
+    ScheduledStepsPhi
+      (initial_state heap env rho e)
+      phi
+      (StDone heap' v) ->
+    exists stty',
+      StoreExtends stty stty' /\
+      TcHeap (heap', stty') /\
+      RuntimeHeapShape heap' stty' /\
+      TcVal (stty', v, subst_rho rho t) /\
+      RuntimeValShape stty' (subst_rho rho t) v /\
+      TcPhi stty' phi.
+Proof.
+  intros heap env rho e stty ctxt rgns t eff phi heap' v
+    HTcHeap HHeapShape HTcRho HTcInc HTcEnv HEnvShape HTcExp HSteps.
+  eapply WTStateRuntimeHeapShapeAt_scheduled_terminal_value_with_trace; eauto.
+  eapply WTStateRuntimeHeapShapeAt_initial; eauto.
+Qed.
+
 Theorem PaperSmallStepTerminalDeterminism :
   forall state trace1 heap1 v1 trace2 heap2 v2,
     Steps state trace1 (StDone heap1 v1) ->
@@ -229,6 +473,30 @@ Proof.
   exact StepsPhi_terminal_deterministic.
 Qed.
 
+Theorem PaperScheduledSmallStepTerminalDeterminism :
+  forall state phi1 heap1 v1 phi2 heap2 v2,
+    ScheduledStepsPhi state phi1 (StDone heap1 v1) ->
+    ScheduledStepsPhi state phi2 (StDone heap2 v2) ->
+    heap1 = heap2 /\ v1 = v2.
+Proof.
+  exact ScheduledStepsPhi_terminal_deterministic.
+Qed.
+
+Theorem PaperScheduledExpressionTerminalDeterminism :
+  forall heap env rho e phi1 heap1 v1 phi2 heap2 v2,
+    ScheduledStepsPhi
+      (initial_state heap env rho e)
+      phi1
+      (StDone heap1 v1) ->
+    ScheduledStepsPhi
+      (initial_state heap env rho e)
+      phi2
+      (StDone heap2 v2) ->
+    heap1 = heap2 /\ v1 = v2.
+Proof.
+  exact ScheduledInitialState_terminal_deterministic.
+Qed.
+
 Theorem PaperSmallStepStructuredEffectTerminalDeterminism :
   forall state phi1 heap1 theta1 phi2 heap2 theta2,
     StepsPhi state phi1 (StDone heap1 (Eff theta1)) ->
@@ -238,31 +506,4 @@ Theorem PaperSmallStepStructuredEffectTerminalDeterminism :
     theta1 = theta2.
 Proof.
   exact StepsPhi_effect_terminal_deterministic.
-Qed.
-
-Theorem PaperPairParCheckedArbitraryScheduleTerminalDeterminism :
-  forall heap env rho ef1 ea1 ef2 ea2
-    phi_state1 phi_left1 phi_right1
-    phi_state2 phi_left2 phi_right2
-    heap1 heap2 v1 v2 theta_left theta_right,
-    PairParCheckPass theta_left theta_right ->
-    phi_left1 ⋞ theta_left ->
-    phi_right1 ⋞ theta_right ->
-    phi_left2 ⋞ theta_left ->
-    phi_right2 ⋞ theta_right ->
-    PairParStepsPhi
-      (pairpar_checked_start heap env rho ef1 ea1 ef2 ea2 KDone)
-      phi_state1
-      phi_left1
-      phi_right1
-      (PPS_State (StDone heap1 v1)) ->
-    PairParStepsPhi
-      (pairpar_checked_start heap env rho ef1 ea1 ef2 ea2 KDone)
-      phi_state2
-      phi_left2
-      phi_right2
-      (PPS_State (StDone heap2 v2)) ->
-    heap1 = heap2 /\ v1 = v2.
-Proof.
-  exact PairParCheckedArbitraryScheduleTerminalDeterminism.
 Qed.
